src/lang/Time.v
@@ -21,7 +21,92 @@ Module Time.
     apply le_lteq in BC. des; subst; auto.
     etransitivity; eauto.
   Qed.
+
+  Lemma le_lt_lt a b c
+        (AB: le a b)
+        (BC: lt b c):
+    lt a c.
+  Proof.
+    apply le_lteq in AB. des; subst; auto.
+    etransitivity; eauto.
+  Qed.
+
+  Lemma le_lt_dec (lhs rhs:t): {le lhs rhs} + {lt rhs lhs}.
+  Proof.
+    generalize (compare_spec lhs rhs).
+    destruct (compare lhs rhs).
+    - left. inv H. reflexivity.
+    - left. inv H. apply Time.le_lteq. auto.
+    - right. inv H. auto.
+  Defined.
+
+  Definition max (lhs rhs:t): t :=
+    match compare lhs rhs with
+    | Lt | Eq => rhs
+    | Gt => lhs
+    end.
+
+  Lemma max_lhs lhs rhs:
+    le lhs (max lhs rhs).
+  Proof.
+    unfold max. destruct (compare_spec lhs rhs).
+    - subst. reflexivity.
+    - apply le_lteq. auto.
+    - reflexivity.
+  Qed.
+
+  Lemma max_rhs lhs rhs:
+    le rhs (max lhs rhs).
+  Proof.
+    unfold max. destruct (compare_spec lhs rhs).
+    - reflexivity.
+    - reflexivity.
+    - apply le_lteq. auto.
+  Qed.
+
+  Lemma max_spec lhs rhs o
+        (LHS: le lhs o)
+        (RHS: le rhs o):
+    le (max lhs rhs) o.
+  Proof.
+    unfold max. destruct (compare_spec lhs rhs); auto.
+  Qed.
+
+  Lemma max_spec' lhs rhs o
+        (LHS: lt lhs o)
+        (RHS: lt rhs o):
+    lt (max lhs rhs) o.
+  Proof.
+    unfold max. destruct (compare_spec lhs rhs); auto.
+  Qed.
+
 End Time.
+
+Ltac timetac :=
+  repeat
+    (try match goal with
+         | [H: Some _ = None |- _] => inv H
+         | [H: None = Some _ |- _] => inv H
+         | [H: ?x <> ?x |- _] => by contradict H
+         | [H: Time.lt ?x ?x |- _] =>
+           apply Time.lt_strorder in H; by inv H
+         | [H1: Time.lt ?a ?b, H2: Time.le ?b ?c |- _] =>
+           exploit (@Time.lt_le_lt a b c); eauto;
+           let H := fresh "H" in
+           intro H; apply Time.lt_strorder in H; by inv H
+
+         | [H: Some _ = Some _ |- _] => inv H
+
+         | [H: context[Time.eq_dec ?a ?b] |- _] =>
+           destruct (Time.eq_dec a b)
+         | [H: context[Time.le_lt_dec ?a ?b] |- _] =>
+           destruct (Time.le_lt_dec a b)
+         | [|- context[Time.eq_dec ?a ?b]] =>
+           destruct (Time.eq_dec a b)
+         | [|- context[Time.le_lt_dec ?a ?b]] =>
+           destruct (Time.le_lt_dec a b)
+         end;
+     ss; subst; auto).
 
 Module TimeSet := UsualSet Time.
 Module TimeFun := UsualFun Time.
@@ -34,6 +119,16 @@ Module Interval <: UsualOrderedType.
       (FROM: Time.lt interval.(fst) x)
       (TO: Time.le x interval.(snd))
   .
+
+  Lemma mem_dec i x: {mem i x} + {~ mem i x}.
+  Proof.
+    destruct i as [lb ub].
+    destruct (Time.le_lt_dec x lb).
+    - right. intro X. inv X. ss. timetac.
+    - destruct (Time.le_lt_dec x ub).
+      + left. econs; s; auto.
+      + right. intro X. inv X. ss. timetac.
+  Defined.
 
   Definition disjoint (lhs rhs:t): Prop :=
     forall x
