src/lib/Axioms.v
@@ -1,6 +1,3 @@
 Require Export Classical.
+Require Export ClassicalChoice.
 Require Export FunctionalExtensionality.
-
-Axiom prop_ext:
-  forall (P Q : Prop), 
-    (P <-> Q) -> P = Q.
