src/lib/Basic.v
@@ -63,3 +63,8 @@ Proof.
     econs; eauto.
   - left. eexists. splits; eauto.
 Qed.
+
+Lemma fapp A (B:A->Type) (a:A) (P Q:forall (a:A), B a)
+      (EQ: P = Q):
+  P a = Q a.
+Proof. rewrite EQ. auto. Qed.
